spec/Address.ec
@@ -22,7 +22,7 @@ qed.
 (* FIXME: REMOVE THIS FROM HERE *)
 
 module M = {
- proc _zero_address (addr:W32.t Array8.t) : W32.t Array8.t = {
+  proc _zero_address (addr:W32.t Array8.t) : W32.t Array8.t = {
     var aux: int;
     
     var i:int;
@@ -211,15 +211,9 @@ lemma set_layer_addr_op_impl (addr : adrs, layer: int):
     set_layer_addr_pre layer => 
         hoare[M.__set_layer_addr : 
             arg = (addr, W32.of_int layer) ==> res = set_layer_addr addr layer].
-proof.
-move => pre_cond.
-proc.
-wp.
-progress.
-qed.
+proof. move => pre_cond. proc. auto. qed.
 
 pred set_tree_addr_pre (tree_address : int) = 0 <= tree_address.
-
 op set_tree_addr (address : adrs, tree_address : int) : adrs = 
 (* 
 FIXME: Should use >> instead of SHR_64.`6 but I cant prove it
@@ -233,12 +227,7 @@ lemma set_tree_addr_op_impl (address : adrs, tree_address : int):
         hoare[M.__set_tree_addr : 
             arg = (address, W64.of_int tree_address) ==> res = set_tree_addr address tree_address].
 
-proof.
-move => pre_cond.
-proc.
-wp.
-progress.
-qed.
+proof. move => pre_cond. proc. auto. qed.
 
 pred set_type_pre (_type : int) = 0 <= _type <= 2.
 op set_type (address : adrs, _type : int) : adrs = 
@@ -247,12 +236,7 @@ lemma set_type_op_impl (address : adrs, _type : int):
     set_type_pre _type =>
         hoare[M.__set_type :
             arg = (address, W32.of_int _type) ==> res = set_type address _type].
-proof.
-move => pre_cond.
-proc.
-wp.
-progress.
-qed.
+proof. move => pre_cond. proc. auto. qed.
 
 
 (* TODO: Add Precondition *)
@@ -261,11 +245,7 @@ op set_ots_addr (address : adrs, ots_addr : int) : adrs =
 lemma set_ots_addr_op_impl (address : adrs, ots_addr : int):
     hoare[M.__set_ots_addr :
         arg = (address, W32.of_int ots_addr) ==> res = set_ots_addr address ots_addr].
-proof.
-proc.
-wp.
-progress.
-qed.
+proof. proc. auto. qed.
 
 
 (* TODO: Add Precondition *)
@@ -274,12 +254,7 @@ op set_chain_addr (address : adrs, chain_addr : int) : adrs =
 lemma set_chain_addr_op_impl (address : adrs, chain_addr : int):
     hoare[M.__set_chain_addr :
         arg = (address, W32.of_int chain_addr) ==> res = set_chain_addr address chain_addr].
-proof.
-proc.
-wp.
-progress.
-qed.
-
+proof. proc. auto. qed.
 
 (* TODO: Add Precondition *)
 op set_hash_addr (address : adrs, hash_addr : int) : adrs = 
@@ -287,12 +262,7 @@ op set_hash_addr (address : adrs, hash_addr : int) : adrs =
 lemma set_hash_addr_op_impl (address : adrs, hash_addr : int):
     hoare[M.__set_hash_addr :
         arg = (address, W32.of_int hash_addr) ==> res = set_hash_addr address hash_addr].
-proof.
-proc.
-wp.
-progress.
-qed.
-
+proof. proc. auto. qed.
 
 (* TODO: Add Precondition *)
 op set_ltree_addr (address : adrs, ltree_addr : int) : adrs = 
@@ -300,18 +270,11 @@ op set_ltree_addr (address : adrs, ltree_addr : int) : adrs =
 lemma set_ltree_addr_op_impl (address : adrs, ltree_addr : int):
     hoare[M.__set_ltree_addr :
         arg = (address, W32.of_int ltree_addr) ==> res = set_ltree_addr address ltree_addr].
-proof.
-proc.
-wp.
-progress.
-qed.
-
+proof. proc. auto. qed.
 
 pred tree_height_pre (tree_height : int) = 0 <= tree_height <= XMSS_TREE_HEIGHT. 
-
 op set_tree_height (address : adrs, tree_height : int) : adrs = 
     address.[5 <- W32.of_int tree_height].
-
 op get_tree_height (address : adrs) : int =
   W32.to_uint (address.[5]).
 
@@ -319,12 +282,7 @@ lemma set_tree_height_op_impl (address : adrs, tree_height : int):
     tree_height_pre tree_height =>
         hoare[M.__set_tree_height :
             arg = (address, W32.of_int tree_height) ==> res = set_tree_height address tree_height].
-proof.
-move => pre_cond.
-proc.
-wp.
-progress.
-qed.
+proof. move => pre_cond. proc. auto. qed.
 
 lemma get_set_tree_height (address : adrs, tree_height : int) :
     tree_height_pre tree_height => 
@@ -333,7 +291,7 @@ proof.
 rewrite /get_tree_height /set_tree_height.
 progress.
 apply word_int.
-progress by (elim H ; smt).
+smt().
 qed.
 
 (* TODO: Add Precondition *)
@@ -345,11 +303,7 @@ op get_tree_index (address : adrs) : int = to_uint (address.[6]).
 lemma set_tree_index_op_impl (address : adrs, tree_index) : 
     hoare[M.__set_tree_index :
         arg = (address, W32.of_int tree_index) ==> res = set_tree_index address tree_index].
-proof.
-proc.
-wp.
-progress.
-qed.
+proof. proc. auto. qed.
 
 lemma get_set_tree_index (address : adrs, tree_index : int) :
   0 <= tree_index < W32.modulus => (* i.e. tree_index fits in a u32 *)
@@ -358,7 +312,7 @@ proof.
 rewrite /get_tree_index /set_tree_index.
 progress.
 apply word_int.
-progress by (elim H; smt).
+ smt().
 qed.
 
 
@@ -367,11 +321,7 @@ op set_key_and_mask (address : adrs, key_and_mask : int) : adrs =
 lemma set_key_and_mask_op_impl (address : adrs, key_and_mask : int):
     hoare[M.__set_key_and_mask :
         arg = (address, W32.of_int key_and_mask) ==> res = set_key_and_mask address key_and_mask].
-proof.
-proc.
-wp.
-progress.
-qed.
+proof. proc. auto. qed.
 
 op zero_addr : adrs = Array8.init (fun _ => W32.zero). 
 lemma zero_addr_op_impl (address : adrs) :
