spec/Properties.ec
@@ -1,0 +1,29 @@
+pragma Goals : printall.
+
+
+require import AllCore List Distr RealExp IntDiv.
+require (*  *) Subtype.
+
+from Jasmin require import JModel.
+
+require import Notation Address Primitives Wots.
+
+import DList.
+import NBytes.
+
+(******************************************************************************)
+
+(* Given a list [(a, b)], maps f over 'a's *)
+(* Same as map (first f) in Haskell        *)
+op map1 ['a] (f : nbytes -> nbytes) (xs : (nbytes * nbytes) list) =
+    with xs = [] => []
+    with xs = h::t => (f h.`1, h.`2) :: (map1 f t).
+
+
+op from_int_list (x : int list) : byte list = map W8.of_int x.
+
+(******************************************************************************)
+
+op sample_n_bytes : nbytes distr = DList.dlist W8.dword n.
+
+op genSKWots : wots_sk distr = DList.dlist sample_n_bytes len.
